Update to autosubst-ocaml

syntax.sig
@@ -2,6 +2,6 @@ tm : Type
 nat : Type
 
 Univ : nat -> tm
-Lam : tm -> (tm -> tm) -> tm
-App : tm -> (tm -> tm) -> tm -> tm -> tm
-Pi : tm -> (tm -> tm) -> tm
+Lam : tm -> (bind tm in tm) -> tm
+App : tm -> (bind tm in tm) -> tm -> tm -> tm
+Pi : tm -> (bind tm in tm) -> tm
