theories/Autosubst2/syntax.v
@@ -1,263 +1,607 @@
-Require Export unscoped.
+Require Import core unscoped.
+
+Require Import Setoid Morphisms Relation_Definitions.
 
 
+Module Core.
 
+Inductive tm : Type :=
+  | var_tm : nat -> tm
+  | Univ : nat -> tm
+  | Lam : tm -> tm -> tm
+  | App : tm -> tm -> tm -> tm -> tm
+  | Pi : tm -> tm -> tm.
 
-Section tm.
-Inductive tm  : Type :=
-  | var_tm : ( fin ) -> tm 
-  | Univ : ( nat   ) -> tm 
-  | Lam : ( tm   ) -> ( tm   ) -> tm 
-  | App : ( tm   ) -> ( tm   ) -> ( tm   ) -> ( tm   ) -> tm 
-  | Pi : ( tm   ) -> ( tm   ) -> tm .
+Lemma congr_Univ {s0 : nat} {t0 : nat} (H0 : s0 = t0) : Univ s0 = Univ t0.
+Proof.
+exact (eq_trans eq_refl (ap (fun x => Univ x) H0)).
+Qed.
 
-Lemma congr_Univ  { s0 : nat   } { t0 : nat   } (H1 : s0 = t0) : Univ  s0 = Univ  t0 .
-Proof. congruence. Qed.
+Lemma congr_Lam {s0 : tm} {s1 : tm} {t0 : tm} {t1 : tm} (H0 : s0 = t0)
+  (H1 : s1 = t1) : Lam s0 s1 = Lam t0 t1.
+Proof.
+exact (eq_trans (eq_trans eq_refl (ap (fun x => Lam x s1) H0))
+         (ap (fun x => Lam t0 x) H1)).
+Qed.
 
-Lemma congr_Lam  { s0 : tm   } { s1 : tm   } { t0 : tm   } { t1 : tm   } (H1 : s0 = t0) (H2 : s1 = t1) : Lam  s0 s1 = Lam  t0 t1 .
-Proof. congruence. Qed.
+Lemma congr_App {s0 : tm} {s1 : tm} {s2 : tm} {s3 : tm} {t0 : tm} {t1 : tm}
+  {t2 : tm} {t3 : tm} (H0 : s0 = t0) (H1 : s1 = t1) (H2 : s2 = t2)
+  (H3 : s3 = t3) : App s0 s1 s2 s3 = App t0 t1 t2 t3.
+Proof.
+exact (eq_trans
+         (eq_trans
+            (eq_trans (eq_trans eq_refl (ap (fun x => App x s1 s2 s3) H0))
+               (ap (fun x => App t0 x s2 s3) H1))
+            (ap (fun x => App t0 t1 x s3) H2))
+         (ap (fun x => App t0 t1 t2 x) H3)).
+Qed.
 
-Lemma congr_App  { s0 : tm   } { s1 : tm   } { s2 : tm   } { s3 : tm   } { t0 : tm   } { t1 : tm   } { t2 : tm   } { t3 : tm   } (H1 : s0 = t0) (H2 : s1 = t1) (H3 : s2 = t2) (H4 : s3 = t3) : App  s0 s1 s2 s3 = App  t0 t1 t2 t3 .
-Proof. congruence. Qed.
+Lemma congr_Pi {s0 : tm} {s1 : tm} {t0 : tm} {t1 : tm} (H0 : s0 = t0)
+  (H1 : s1 = t1) : Pi s0 s1 = Pi t0 t1.
+Proof.
+exact (eq_trans (eq_trans eq_refl (ap (fun x => Pi x s1) H0))
+         (ap (fun x => Pi t0 x) H1)).
+Qed.
 
-Lemma congr_Pi  { s0 : tm   } { s1 : tm   } { t0 : tm   } { t1 : tm   } (H1 : s0 = t0) (H2 : s1 = t1) : Pi  s0 s1 = Pi  t0 t1 .
-Proof. congruence. Qed.
+Lemma upRen_tm_tm (xi : nat -> nat) : nat -> nat.
+Proof.
+exact (up_ren xi).
+Defined.
 
-Definition upRen_tm_tm   (xi : ( fin ) -> fin) : ( fin ) -> fin :=
-  (up_ren) xi.
-
-Fixpoint ren_tm   (xitm : ( fin ) -> fin) (s : tm ) : tm  :=
-    match s return tm  with
-    | var_tm  s => (var_tm ) (xitm s)
-    | Univ  s0 => Univ  ((fun x => x) s0)
-    | Lam  s0 s1 => Lam  ((ren_tm xitm) s0) ((ren_tm (upRen_tm_tm xitm)) s1)
-    | App  s0 s1 s2 s3 => App  ((ren_tm xitm) s0) ((ren_tm (upRen_tm_tm xitm)) s1) ((ren_tm xitm) s2) ((ren_tm xitm) s3)
-    | Pi  s0 s1 => Pi  ((ren_tm xitm) s0) ((ren_tm (upRen_tm_tm xitm)) s1)
-    end.
-
-Definition up_tm_tm   (sigma : ( fin ) -> tm ) : ( fin ) -> tm  :=
-  (scons) ((var_tm ) (var_zero)) ((funcomp) (ren_tm (shift)) sigma).
-
-Fixpoint subst_tm   (sigmatm : ( fin ) -> tm ) (s : tm ) : tm  :=
-    match s return tm  with
-    | var_tm  s => sigmatm s
-    | Univ  s0 => Univ  ((fun x => x) s0)
-    | Lam  s0 s1 => Lam  ((subst_tm sigmatm) s0) ((subst_tm (up_tm_tm sigmatm)) s1)
-    | App  s0 s1 s2 s3 => App  ((subst_tm sigmatm) s0) ((subst_tm (up_tm_tm sigmatm)) s1) ((subst_tm sigmatm) s2) ((subst_tm sigmatm) s3)
-    | Pi  s0 s1 => Pi  ((subst_tm sigmatm) s0) ((subst_tm (up_tm_tm sigmatm)) s1)
-    end.
-
-Definition upId_tm_tm  (sigma : ( fin ) -> tm ) (Eq : forall x, sigma x = (var_tm ) x) : forall x, (up_tm_tm sigma) x = (var_tm ) x :=
-  fun n => match n with
-  | S fin_n => (ap) (ren_tm (shift)) (Eq fin_n)
-  | 0  => eq_refl
+Fixpoint ren_tm (xi_tm : nat -> nat) (s : tm) {struct s} : tm :=
+  match s with
+  | var_tm s0 => var_tm (xi_tm s0)
+  | Univ s0 => Univ s0
+  | Lam s0 s1 => Lam (ren_tm xi_tm s0) (ren_tm (upRen_tm_tm xi_tm) s1)
+  | App s0 s1 s2 s3 =>
+      App (ren_tm xi_tm s0) (ren_tm (upRen_tm_tm xi_tm) s1) (ren_tm xi_tm s2)
+        (ren_tm xi_tm s3)
+  | Pi s0 s1 => Pi (ren_tm xi_tm s0) (ren_tm (upRen_tm_tm xi_tm) s1)
   end.
 
-Fixpoint idSubst_tm  (sigmatm : ( fin ) -> tm ) (Eqtm : forall x, sigmatm x = (var_tm ) x) (s : tm ) : subst_tm sigmatm s = s :=
-    match s return subst_tm sigmatm s = s with
-    | var_tm  s => Eqtm s
-    | Univ  s0 => congr_Univ ((fun x => (eq_refl) x) s0)
-    | Lam  s0 s1 => congr_Lam ((idSubst_tm sigmatm Eqtm) s0) ((idSubst_tm (up_tm_tm sigmatm) (upId_tm_tm (_) Eqtm)) s1)
-    | App  s0 s1 s2 s3 => congr_App ((idSubst_tm sigmatm Eqtm) s0) ((idSubst_tm (up_tm_tm sigmatm) (upId_tm_tm (_) Eqtm)) s1) ((idSubst_tm sigmatm Eqtm) s2) ((idSubst_tm sigmatm Eqtm) s3)
-    | Pi  s0 s1 => congr_Pi ((idSubst_tm sigmatm Eqtm) s0) ((idSubst_tm (up_tm_tm sigmatm) (upId_tm_tm (_) Eqtm)) s1)
-    end.
+Lemma up_tm_tm (sigma : nat -> tm) : nat -> tm.
+Proof.
+exact (scons (var_tm var_zero) (funcomp (ren_tm shift) sigma)).
+Defined.
 
-Definition upExtRen_tm_tm   (xi : ( fin ) -> fin) (zeta : ( fin ) -> fin) (Eq : forall x, xi x = zeta x) : forall x, (upRen_tm_tm xi) x = (upRen_tm_tm zeta) x :=
-  fun n => match n with
-  | S fin_n => (ap) (shift) (Eq fin_n)
-  | 0  => eq_refl
+Fixpoint subst_tm (sigma_tm : nat -> tm) (s : tm) {struct s} : tm :=
+  match s with
+  | var_tm s0 => sigma_tm s0
+  | Univ s0 => Univ s0
+  | Lam s0 s1 => Lam (subst_tm sigma_tm s0) (subst_tm (up_tm_tm sigma_tm) s1)
+  | App s0 s1 s2 s3 =>
+      App (subst_tm sigma_tm s0) (subst_tm (up_tm_tm sigma_tm) s1)
+        (subst_tm sigma_tm s2) (subst_tm sigma_tm s3)
+  | Pi s0 s1 => Pi (subst_tm sigma_tm s0) (subst_tm (up_tm_tm sigma_tm) s1)
   end.
 
-Fixpoint extRen_tm   (xitm : ( fin ) -> fin) (zetatm : ( fin ) -> fin) (Eqtm : forall x, xitm x = zetatm x) (s : tm ) : ren_tm xitm s = ren_tm zetatm s :=
-    match s return ren_tm xitm s = ren_tm zetatm s with
-    | var_tm  s => (ap) (var_tm ) (Eqtm s)
-    | Univ  s0 => congr_Univ ((fun x => (eq_refl) x) s0)
-    | Lam  s0 s1 => congr_Lam ((extRen_tm xitm zetatm Eqtm) s0) ((extRen_tm (upRen_tm_tm xitm) (upRen_tm_tm zetatm) (upExtRen_tm_tm (_) (_) Eqtm)) s1)
-    | App  s0 s1 s2 s3 => congr_App ((extRen_tm xitm zetatm Eqtm) s0) ((extRen_tm (upRen_tm_tm xitm) (upRen_tm_tm zetatm) (upExtRen_tm_tm (_) (_) Eqtm)) s1) ((extRen_tm xitm zetatm Eqtm) s2) ((extRen_tm xitm zetatm Eqtm) s3)
-    | Pi  s0 s1 => congr_Pi ((extRen_tm xitm zetatm Eqtm) s0) ((extRen_tm (upRen_tm_tm xitm) (upRen_tm_tm zetatm) (upExtRen_tm_tm (_) (_) Eqtm)) s1)
-    end.
+Lemma upId_tm_tm (sigma : nat -> tm) (Eq : forall x, sigma x = var_tm x) :
+  forall x, up_tm_tm sigma x = var_tm x.
+Proof.
+exact (fun n =>
+       match n with
+       | S n' => ap (ren_tm shift) (Eq n')
+       | O => eq_refl
+       end).
+Qed.
 
-Definition upExt_tm_tm   (sigma : ( fin ) -> tm ) (tau : ( fin ) -> tm ) (Eq : forall x, sigma x = tau x) : forall x, (up_tm_tm sigma) x = (up_tm_tm tau) x :=
-  fun n => match n with
-  | S fin_n => (ap) (ren_tm (shift)) (Eq fin_n)
-  | 0  => eq_refl
+Fixpoint idSubst_tm (sigma_tm : nat -> tm)
+(Eq_tm : forall x, sigma_tm x = var_tm x) (s : tm) {struct s} :
+subst_tm sigma_tm s = s :=
+  match s with
+  | var_tm s0 => Eq_tm s0
+  | Univ s0 => congr_Univ (eq_refl s0)
+  | Lam s0 s1 =>
+      congr_Lam (idSubst_tm sigma_tm Eq_tm s0)
+        (idSubst_tm (up_tm_tm sigma_tm) (upId_tm_tm _ Eq_tm) s1)
+  | App s0 s1 s2 s3 =>
+      congr_App (idSubst_tm sigma_tm Eq_tm s0)
+        (idSubst_tm (up_tm_tm sigma_tm) (upId_tm_tm _ Eq_tm) s1)
+        (idSubst_tm sigma_tm Eq_tm s2) (idSubst_tm sigma_tm Eq_tm s3)
+  | Pi s0 s1 =>
+      congr_Pi (idSubst_tm sigma_tm Eq_tm s0)
+        (idSubst_tm (up_tm_tm sigma_tm) (upId_tm_tm _ Eq_tm) s1)
   end.
 
-Fixpoint ext_tm   (sigmatm : ( fin ) -> tm ) (tautm : ( fin ) -> tm ) (Eqtm : forall x, sigmatm x = tautm x) (s : tm ) : subst_tm sigmatm s = subst_tm tautm s :=
-    match s return subst_tm sigmatm s = subst_tm tautm s with
-    | var_tm  s => Eqtm s
-    | Univ  s0 => congr_Univ ((fun x => (eq_refl) x) s0)
-    | Lam  s0 s1 => congr_Lam ((ext_tm sigmatm tautm Eqtm) s0) ((ext_tm (up_tm_tm sigmatm) (up_tm_tm tautm) (upExt_tm_tm (_) (_) Eqtm)) s1)
-    | App  s0 s1 s2 s3 => congr_App ((ext_tm sigmatm tautm Eqtm) s0) ((ext_tm (up_tm_tm sigmatm) (up_tm_tm tautm) (upExt_tm_tm (_) (_) Eqtm)) s1) ((ext_tm sigmatm tautm Eqtm) s2) ((ext_tm sigmatm tautm Eqtm) s3)
-    | Pi  s0 s1 => congr_Pi ((ext_tm sigmatm tautm Eqtm) s0) ((ext_tm (up_tm_tm sigmatm) (up_tm_tm tautm) (upExt_tm_tm (_) (_) Eqtm)) s1)
-    end.
+Lemma upExtRen_tm_tm (xi : nat -> nat) (zeta : nat -> nat)
+  (Eq : forall x, xi x = zeta x) :
+  forall x, upRen_tm_tm xi x = upRen_tm_tm zeta x.
+Proof.
+exact (fun n => match n with
+                | S n' => ap shift (Eq n')
+                | O => eq_refl
+                end).
+Qed.
 
-Definition up_ren_ren_tm_tm    (xi : ( fin ) -> fin) (tau : ( fin ) -> fin) (theta : ( fin ) -> fin) (Eq : forall x, ((funcomp) tau xi) x = theta x) : forall x, ((funcomp) (upRen_tm_tm tau) (upRen_tm_tm xi)) x = (upRen_tm_tm theta) x :=
-  up_ren_ren xi tau theta Eq.
-
-Fixpoint compRenRen_tm    (xitm : ( fin ) -> fin) (zetatm : ( fin ) -> fin) (rhotm : ( fin ) -> fin) (Eqtm : forall x, ((funcomp) zetatm xitm) x = rhotm x) (s : tm ) : ren_tm zetatm (ren_tm xitm s) = ren_tm rhotm s :=
-    match s return ren_tm zetatm (ren_tm xitm s) = ren_tm rhotm s with
-    | var_tm  s => (ap) (var_tm ) (Eqtm s)
-    | Univ  s0 => congr_Univ ((fun x => (eq_refl) x) s0)
-    | Lam  s0 s1 => congr_Lam ((compRenRen_tm xitm zetatm rhotm Eqtm) s0) ((compRenRen_tm (upRen_tm_tm xitm) (upRen_tm_tm zetatm) (upRen_tm_tm rhotm) (up_ren_ren (_) (_) (_) Eqtm)) s1)
-    | App  s0 s1 s2 s3 => congr_App ((compRenRen_tm xitm zetatm rhotm Eqtm) s0) ((compRenRen_tm (upRen_tm_tm xitm) (upRen_tm_tm zetatm) (upRen_tm_tm rhotm) (up_ren_ren (_) (_) (_) Eqtm)) s1) ((compRenRen_tm xitm zetatm rhotm Eqtm) s2) ((compRenRen_tm xitm zetatm rhotm Eqtm) s3)
-    | Pi  s0 s1 => congr_Pi ((compRenRen_tm xitm zetatm rhotm Eqtm) s0) ((compRenRen_tm (upRen_tm_tm xitm) (upRen_tm_tm zetatm) (upRen_tm_tm rhotm) (up_ren_ren (_) (_) (_) Eqtm)) s1)
-    end.
-
-Definition up_ren_subst_tm_tm    (xi : ( fin ) -> fin) (tau : ( fin ) -> tm ) (theta : ( fin ) -> tm ) (Eq : forall x, ((funcomp) tau xi) x = theta x) : forall x, ((funcomp) (up_tm_tm tau) (upRen_tm_tm xi)) x = (up_tm_tm theta) x :=
-  fun n => match n with
-  | S fin_n => (ap) (ren_tm (shift)) (Eq fin_n)
-  | 0  => eq_refl
+Fixpoint extRen_tm (xi_tm : nat -> nat) (zeta_tm : nat -> nat)
+(Eq_tm : forall x, xi_tm x = zeta_tm x) (s : tm) {struct s} :
+ren_tm xi_tm s = ren_tm zeta_tm s :=
+  match s with
+  | var_tm s0 => ap (var_tm) (Eq_tm s0)
+  | Univ s0 => congr_Univ (eq_refl s0)
+  | Lam s0 s1 =>
+      congr_Lam (extRen_tm xi_tm zeta_tm Eq_tm s0)
+        (extRen_tm (upRen_tm_tm xi_tm) (upRen_tm_tm zeta_tm)
+           (upExtRen_tm_tm _ _ Eq_tm) s1)
+  | App s0 s1 s2 s3 =>
+      congr_App (extRen_tm xi_tm zeta_tm Eq_tm s0)
+        (extRen_tm (upRen_tm_tm xi_tm) (upRen_tm_tm zeta_tm)
+           (upExtRen_tm_tm _ _ Eq_tm) s1) (extRen_tm xi_tm zeta_tm Eq_tm s2)
+        (extRen_tm xi_tm zeta_tm Eq_tm s3)
+  | Pi s0 s1 =>
+      congr_Pi (extRen_tm xi_tm zeta_tm Eq_tm s0)
+        (extRen_tm (upRen_tm_tm xi_tm) (upRen_tm_tm zeta_tm)
+           (upExtRen_tm_tm _ _ Eq_tm) s1)
   end.
 
-Fixpoint compRenSubst_tm    (xitm : ( fin ) -> fin) (tautm : ( fin ) -> tm ) (thetatm : ( fin ) -> tm ) (Eqtm : forall x, ((funcomp) tautm xitm) x = thetatm x) (s : tm ) : subst_tm tautm (ren_tm xitm s) = subst_tm thetatm s :=
-    match s return subst_tm tautm (ren_tm xitm s) = subst_tm thetatm s with
-    | var_tm  s => Eqtm s
-    | Univ  s0 => congr_Univ ((fun x => (eq_refl) x) s0)
-    | Lam  s0 s1 => congr_Lam ((compRenSubst_tm xitm tautm thetatm Eqtm) s0) ((compRenSubst_tm (upRen_tm_tm xitm) (up_tm_tm tautm) (up_tm_tm thetatm) (up_ren_subst_tm_tm (_) (_) (_) Eqtm)) s1)
-    | App  s0 s1 s2 s3 => congr_App ((compRenSubst_tm xitm tautm thetatm Eqtm) s0) ((compRenSubst_tm (upRen_tm_tm xitm) (up_tm_tm tautm) (up_tm_tm thetatm) (up_ren_subst_tm_tm (_) (_) (_) Eqtm)) s1) ((compRenSubst_tm xitm tautm thetatm Eqtm) s2) ((compRenSubst_tm xitm tautm thetatm Eqtm) s3)
-    | Pi  s0 s1 => congr_Pi ((compRenSubst_tm xitm tautm thetatm Eqtm) s0) ((compRenSubst_tm (upRen_tm_tm xitm) (up_tm_tm tautm) (up_tm_tm thetatm) (up_ren_subst_tm_tm (_) (_) (_) Eqtm)) s1)
-    end.
+Lemma upExt_tm_tm (sigma : nat -> tm) (tau : nat -> tm)
+  (Eq : forall x, sigma x = tau x) :
+  forall x, up_tm_tm sigma x = up_tm_tm tau x.
+Proof.
+exact (fun n =>
+       match n with
+       | S n' => ap (ren_tm shift) (Eq n')
+       | O => eq_refl
+       end).
+Qed.
 
-Definition up_subst_ren_tm_tm    (sigma : ( fin ) -> tm ) (zetatm : ( fin ) -> fin) (theta : ( fin ) -> tm ) (Eq : forall x, ((funcomp) (ren_tm zetatm) sigma) x = theta x) : forall x, ((funcomp) (ren_tm (upRen_tm_tm zetatm)) (up_tm_tm sigma)) x = (up_tm_tm theta) x :=
-  fun n => match n with
-  | S fin_n => (eq_trans) (compRenRen_tm (shift) (upRen_tm_tm zetatm) ((funcomp) (shift) zetatm) (fun x => eq_refl) (sigma fin_n)) ((eq_trans) ((eq_sym) (compRenRen_tm zetatm (shift) ((funcomp) (shift) zetatm) (fun x => eq_refl) (sigma fin_n))) ((ap) (ren_tm (shift)) (Eq fin_n)))
-  | 0  => eq_refl
+Fixpoint ext_tm (sigma_tm : nat -> tm) (tau_tm : nat -> tm)
+(Eq_tm : forall x, sigma_tm x = tau_tm x) (s : tm) {struct s} :
+subst_tm sigma_tm s = subst_tm tau_tm s :=
+  match s with
+  | var_tm s0 => Eq_tm s0
+  | Univ s0 => congr_Univ (eq_refl s0)
+  | Lam s0 s1 =>
+      congr_Lam (ext_tm sigma_tm tau_tm Eq_tm s0)
+        (ext_tm (up_tm_tm sigma_tm) (up_tm_tm tau_tm) (upExt_tm_tm _ _ Eq_tm)
+           s1)
+  | App s0 s1 s2 s3 =>
+      congr_App (ext_tm sigma_tm tau_tm Eq_tm s0)
+        (ext_tm (up_tm_tm sigma_tm) (up_tm_tm tau_tm) (upExt_tm_tm _ _ Eq_tm)
+           s1) (ext_tm sigma_tm tau_tm Eq_tm s2)
+        (ext_tm sigma_tm tau_tm Eq_tm s3)
+  | Pi s0 s1 =>
+      congr_Pi (ext_tm sigma_tm tau_tm Eq_tm s0)
+        (ext_tm (up_tm_tm sigma_tm) (up_tm_tm tau_tm) (upExt_tm_tm _ _ Eq_tm)
+           s1)
   end.
 
-Fixpoint compSubstRen_tm    (sigmatm : ( fin ) -> tm ) (zetatm : ( fin ) -> fin) (thetatm : ( fin ) -> tm ) (Eqtm : forall x, ((funcomp) (ren_tm zetatm) sigmatm) x = thetatm x) (s : tm ) : ren_tm zetatm (subst_tm sigmatm s) = subst_tm thetatm s :=
-    match s return ren_tm zetatm (subst_tm sigmatm s) = subst_tm thetatm s with
-    | var_tm  s => Eqtm s
-    | Univ  s0 => congr_Univ ((fun x => (eq_refl) x) s0)
-    | Lam  s0 s1 => congr_Lam ((compSubstRen_tm sigmatm zetatm thetatm Eqtm) s0) ((compSubstRen_tm (up_tm_tm sigmatm) (upRen_tm_tm zetatm) (up_tm_tm thetatm) (up_subst_ren_tm_tm (_) (_) (_) Eqtm)) s1)
-    | App  s0 s1 s2 s3 => congr_App ((compSubstRen_tm sigmatm zetatm thetatm Eqtm) s0) ((compSubstRen_tm (up_tm_tm sigmatm) (upRen_tm_tm zetatm) (up_tm_tm thetatm) (up_subst_ren_tm_tm (_) (_) (_) Eqtm)) s1) ((compSubstRen_tm sigmatm zetatm thetatm Eqtm) s2) ((compSubstRen_tm sigmatm zetatm thetatm Eqtm) s3)
-    | Pi  s0 s1 => congr_Pi ((compSubstRen_tm sigmatm zetatm thetatm Eqtm) s0) ((compSubstRen_tm (up_tm_tm sigmatm) (upRen_tm_tm zetatm) (up_tm_tm thetatm) (up_subst_ren_tm_tm (_) (_) (_) Eqtm)) s1)
-    end.
+Lemma up_ren_ren_tm_tm (xi : nat -> nat) (zeta : nat -> nat)
+  (rho : nat -> nat) (Eq : forall x, funcomp zeta xi x = rho x) :
+  forall x, funcomp (upRen_tm_tm zeta) (upRen_tm_tm xi) x = upRen_tm_tm rho x.
+Proof.
+exact (up_ren_ren xi zeta rho Eq).
+Qed.
 
-Definition up_subst_subst_tm_tm    (sigma : ( fin ) -> tm ) (tautm : ( fin ) -> tm ) (theta : ( fin ) -> tm ) (Eq : forall x, ((funcomp) (subst_tm tautm) sigma) x = theta x) : forall x, ((funcomp) (subst_tm (up_tm_tm tautm)) (up_tm_tm sigma)) x = (up_tm_tm theta) x :=
-  fun n => match n with
-  | S fin_n => (eq_trans) (compRenSubst_tm (shift) (up_tm_tm tautm) ((funcomp) (up_tm_tm tautm) (shift)) (fun x => eq_refl) (sigma fin_n)) ((eq_trans) ((eq_sym) (compSubstRen_tm tautm (shift) ((funcomp) (ren_tm (shift)) tautm) (fun x => eq_refl) (sigma fin_n))) ((ap) (ren_tm (shift)) (Eq fin_n)))
-  | 0  => eq_refl
+Fixpoint compRenRen_tm (xi_tm : nat -> nat) (zeta_tm : nat -> nat)
+(rho_tm : nat -> nat) (Eq_tm : forall x, funcomp zeta_tm xi_tm x = rho_tm x)
+(s : tm) {struct s} : ren_tm zeta_tm (ren_tm xi_tm s) = ren_tm rho_tm s :=
+  match s with
+  | var_tm s0 => ap (var_tm) (Eq_tm s0)
+  | Univ s0 => congr_Univ (eq_refl s0)
+  | Lam s0 s1 =>
+      congr_Lam (compRenRen_tm xi_tm zeta_tm rho_tm Eq_tm s0)
+        (compRenRen_tm (upRen_tm_tm xi_tm) (upRen_tm_tm zeta_tm)
+           (upRen_tm_tm rho_tm) (up_ren_ren _ _ _ Eq_tm) s1)
+  | App s0 s1 s2 s3 =>
+      congr_App (compRenRen_tm xi_tm zeta_tm rho_tm Eq_tm s0)
+        (compRenRen_tm (upRen_tm_tm xi_tm) (upRen_tm_tm zeta_tm)
+           (upRen_tm_tm rho_tm) (up_ren_ren _ _ _ Eq_tm) s1)
+        (compRenRen_tm xi_tm zeta_tm rho_tm Eq_tm s2)
+        (compRenRen_tm xi_tm zeta_tm rho_tm Eq_tm s3)
+  | Pi s0 s1 =>
+      congr_Pi (compRenRen_tm xi_tm zeta_tm rho_tm Eq_tm s0)
+        (compRenRen_tm (upRen_tm_tm xi_tm) (upRen_tm_tm zeta_tm)
+           (upRen_tm_tm rho_tm) (up_ren_ren _ _ _ Eq_tm) s1)
   end.
 
-Fixpoint compSubstSubst_tm    (sigmatm : ( fin ) -> tm ) (tautm : ( fin ) -> tm ) (thetatm : ( fin ) -> tm ) (Eqtm : forall x, ((funcomp) (subst_tm tautm) sigmatm) x = thetatm x) (s : tm ) : subst_tm tautm (subst_tm sigmatm s) = subst_tm thetatm s :=
-    match s return subst_tm tautm (subst_tm sigmatm s) = subst_tm thetatm s with
-    | var_tm  s => Eqtm s
-    | Univ  s0 => congr_Univ ((fun x => (eq_refl) x) s0)
-    | Lam  s0 s1 => congr_Lam ((compSubstSubst_tm sigmatm tautm thetatm Eqtm) s0) ((compSubstSubst_tm (up_tm_tm sigmatm) (up_tm_tm tautm) (up_tm_tm thetatm) (up_subst_subst_tm_tm (_) (_) (_) Eqtm)) s1)
-    | App  s0 s1 s2 s3 => congr_App ((compSubstSubst_tm sigmatm tautm thetatm Eqtm) s0) ((compSubstSubst_tm (up_tm_tm sigmatm) (up_tm_tm tautm) (up_tm_tm thetatm) (up_subst_subst_tm_tm (_) (_) (_) Eqtm)) s1) ((compSubstSubst_tm sigmatm tautm thetatm Eqtm) s2) ((compSubstSubst_tm sigmatm tautm thetatm Eqtm) s3)
-    | Pi  s0 s1 => congr_Pi ((compSubstSubst_tm sigmatm tautm thetatm Eqtm) s0) ((compSubstSubst_tm (up_tm_tm sigmatm) (up_tm_tm tautm) (up_tm_tm thetatm) (up_subst_subst_tm_tm (_) (_) (_) Eqtm)) s1)
-    end.
+Lemma up_ren_subst_tm_tm (xi : nat -> nat) (tau : nat -> tm)
+  (theta : nat -> tm) (Eq : forall x, funcomp tau xi x = theta x) :
+  forall x, funcomp (up_tm_tm tau) (upRen_tm_tm xi) x = up_tm_tm theta x.
+Proof.
+exact (fun n =>
+       match n with
+       | S n' => ap (ren_tm shift) (Eq n')
+       | O => eq_refl
+       end).
+Qed.
 
-Definition rinstInst_up_tm_tm   (xi : ( fin ) -> fin) (sigma : ( fin ) -> tm ) (Eq : forall x, ((funcomp) (var_tm ) xi) x = sigma x) : forall x, ((funcomp) (var_tm ) (upRen_tm_tm xi)) x = (up_tm_tm sigma) x :=
-  fun n => match n with
-  | S fin_n => (ap) (ren_tm (shift)) (Eq fin_n)
-  | 0  => eq_refl
+Fixpoint compRenSubst_tm (xi_tm : nat -> nat) (tau_tm : nat -> tm)
+(theta_tm : nat -> tm)
+(Eq_tm : forall x, funcomp tau_tm xi_tm x = theta_tm x) (s : tm) {struct s} :
+subst_tm tau_tm (ren_tm xi_tm s) = subst_tm theta_tm s :=
+  match s with
+  | var_tm s0 => Eq_tm s0
+  | Univ s0 => congr_Univ (eq_refl s0)
+  | Lam s0 s1 =>
+      congr_Lam (compRenSubst_tm xi_tm tau_tm theta_tm Eq_tm s0)
+        (compRenSubst_tm (upRen_tm_tm xi_tm) (up_tm_tm tau_tm)
+           (up_tm_tm theta_tm) (up_ren_subst_tm_tm _ _ _ Eq_tm) s1)
+  | App s0 s1 s2 s3 =>
+      congr_App (compRenSubst_tm xi_tm tau_tm theta_tm Eq_tm s0)
+        (compRenSubst_tm (upRen_tm_tm xi_tm) (up_tm_tm tau_tm)
+           (up_tm_tm theta_tm) (up_ren_subst_tm_tm _ _ _ Eq_tm) s1)
+        (compRenSubst_tm xi_tm tau_tm theta_tm Eq_tm s2)
+        (compRenSubst_tm xi_tm tau_tm theta_tm Eq_tm s3)
+  | Pi s0 s1 =>
+      congr_Pi (compRenSubst_tm xi_tm tau_tm theta_tm Eq_tm s0)
+        (compRenSubst_tm (upRen_tm_tm xi_tm) (up_tm_tm tau_tm)
+           (up_tm_tm theta_tm) (up_ren_subst_tm_tm _ _ _ Eq_tm) s1)
   end.
 
-Fixpoint rinst_inst_tm   (xitm : ( fin ) -> fin) (sigmatm : ( fin ) -> tm ) (Eqtm : forall x, ((funcomp) (var_tm ) xitm) x = sigmatm x) (s : tm ) : ren_tm xitm s = subst_tm sigmatm s :=
-    match s return ren_tm xitm s = subst_tm sigmatm s with
-    | var_tm  s => Eqtm s
-    | Univ  s0 => congr_Univ ((fun x => (eq_refl) x) s0)
-    | Lam  s0 s1 => congr_Lam ((rinst_inst_tm xitm sigmatm Eqtm) s0) ((rinst_inst_tm (upRen_tm_tm xitm) (up_tm_tm sigmatm) (rinstInst_up_tm_tm (_) (_) Eqtm)) s1)
-    | App  s0 s1 s2 s3 => congr_App ((rinst_inst_tm xitm sigmatm Eqtm) s0) ((rinst_inst_tm (upRen_tm_tm xitm) (up_tm_tm sigmatm) (rinstInst_up_tm_tm (_) (_) Eqtm)) s1) ((rinst_inst_tm xitm sigmatm Eqtm) s2) ((rinst_inst_tm xitm sigmatm Eqtm) s3)
-    | Pi  s0 s1 => congr_Pi ((rinst_inst_tm xitm sigmatm Eqtm) s0) ((rinst_inst_tm (upRen_tm_tm xitm) (up_tm_tm sigmatm) (rinstInst_up_tm_tm (_) (_) Eqtm)) s1)
-    end.
+Lemma up_subst_ren_tm_tm (sigma : nat -> tm) (zeta_tm : nat -> nat)
+  (theta : nat -> tm)
+  (Eq : forall x, funcomp (ren_tm zeta_tm) sigma x = theta x) :
+  forall x,
+  funcomp (ren_tm (upRen_tm_tm zeta_tm)) (up_tm_tm sigma) x =
+  up_tm_tm theta x.
+Proof.
+exact (fun n =>
+       match n with
+       | S n' =>
+           eq_trans
+             (compRenRen_tm shift (upRen_tm_tm zeta_tm)
+                (funcomp shift zeta_tm) (fun x => eq_refl) (sigma n'))
+             (eq_trans
+                (eq_sym
+                   (compRenRen_tm zeta_tm shift (funcomp shift zeta_tm)
+                      (fun x => eq_refl) (sigma n')))
+                (ap (ren_tm shift) (Eq n')))
+       | O => eq_refl
+       end).
+Qed.
 
-Lemma rinstInst_tm   (xitm : ( fin ) -> fin) : ren_tm xitm = subst_tm ((funcomp) (var_tm ) xitm) .
-Proof. exact ((FunctionalExtensionality.functional_extensionality _ _ ) (fun x => rinst_inst_tm xitm (_) (fun n => eq_refl) x)). Qed.
+Fixpoint compSubstRen_tm (sigma_tm : nat -> tm) (zeta_tm : nat -> nat)
+(theta_tm : nat -> tm)
+(Eq_tm : forall x, funcomp (ren_tm zeta_tm) sigma_tm x = theta_tm x) 
+(s : tm) {struct s} :
+ren_tm zeta_tm (subst_tm sigma_tm s) = subst_tm theta_tm s :=
+  match s with
+  | var_tm s0 => Eq_tm s0
+  | Univ s0 => congr_Univ (eq_refl s0)
+  | Lam s0 s1 =>
+      congr_Lam (compSubstRen_tm sigma_tm zeta_tm theta_tm Eq_tm s0)
+        (compSubstRen_tm (up_tm_tm sigma_tm) (upRen_tm_tm zeta_tm)
+           (up_tm_tm theta_tm) (up_subst_ren_tm_tm _ _ _ Eq_tm) s1)
+  | App s0 s1 s2 s3 =>
+      congr_App (compSubstRen_tm sigma_tm zeta_tm theta_tm Eq_tm s0)
+        (compSubstRen_tm (up_tm_tm sigma_tm) (upRen_tm_tm zeta_tm)
+           (up_tm_tm theta_tm) (up_subst_ren_tm_tm _ _ _ Eq_tm) s1)
+        (compSubstRen_tm sigma_tm zeta_tm theta_tm Eq_tm s2)
+        (compSubstRen_tm sigma_tm zeta_tm theta_tm Eq_tm s3)
+  | Pi s0 s1 =>
+      congr_Pi (compSubstRen_tm sigma_tm zeta_tm theta_tm Eq_tm s0)
+        (compSubstRen_tm (up_tm_tm sigma_tm) (upRen_tm_tm zeta_tm)
+           (up_tm_tm theta_tm) (up_subst_ren_tm_tm _ _ _ Eq_tm) s1)
+  end.
 
-Lemma instId_tm  : subst_tm (var_tm ) = id .
-Proof. exact ((FunctionalExtensionality.functional_extensionality _ _ ) (fun x => idSubst_tm (var_tm ) (fun n => eq_refl) ((id) x))). Qed.
+Lemma up_subst_subst_tm_tm (sigma : nat -> tm) (tau_tm : nat -> tm)
+  (theta : nat -> tm)
+  (Eq : forall x, funcomp (subst_tm tau_tm) sigma x = theta x) :
+  forall x,
+  funcomp (subst_tm (up_tm_tm tau_tm)) (up_tm_tm sigma) x = up_tm_tm theta x.
+Proof.
+exact (fun n =>
+       match n with
+       | S n' =>
+           eq_trans
+             (compRenSubst_tm shift (up_tm_tm tau_tm)
+                (funcomp (up_tm_tm tau_tm) shift) (fun x => eq_refl)
+                (sigma n'))
+             (eq_trans
+                (eq_sym
+                   (compSubstRen_tm tau_tm shift
+                      (funcomp (ren_tm shift) tau_tm) (fun x => eq_refl)
+                      (sigma n'))) (ap (ren_tm shift) (Eq n')))
+       | O => eq_refl
+       end).
+Qed.
 
-Lemma rinstId_tm  : @ren_tm   (id) = id .
-Proof. exact ((eq_trans) (rinstInst_tm ((id) (_))) instId_tm). Qed.
+Fixpoint compSubstSubst_tm (sigma_tm : nat -> tm) (tau_tm : nat -> tm)
+(theta_tm : nat -> tm)
+(Eq_tm : forall x, funcomp (subst_tm tau_tm) sigma_tm x = theta_tm x)
+(s : tm) {struct s} :
+subst_tm tau_tm (subst_tm sigma_tm s) = subst_tm theta_tm s :=
+  match s with
+  | var_tm s0 => Eq_tm s0
+  | Univ s0 => congr_Univ (eq_refl s0)
+  | Lam s0 s1 =>
+      congr_Lam (compSubstSubst_tm sigma_tm tau_tm theta_tm Eq_tm s0)
+        (compSubstSubst_tm (up_tm_tm sigma_tm) (up_tm_tm tau_tm)
+           (up_tm_tm theta_tm) (up_subst_subst_tm_tm _ _ _ Eq_tm) s1)
+  | App s0 s1 s2 s3 =>
+      congr_App (compSubstSubst_tm sigma_tm tau_tm theta_tm Eq_tm s0)
+        (compSubstSubst_tm (up_tm_tm sigma_tm) (up_tm_tm tau_tm)
+           (up_tm_tm theta_tm) (up_subst_subst_tm_tm _ _ _ Eq_tm) s1)
+        (compSubstSubst_tm sigma_tm tau_tm theta_tm Eq_tm s2)
+        (compSubstSubst_tm sigma_tm tau_tm theta_tm Eq_tm s3)
+  | Pi s0 s1 =>
+      congr_Pi (compSubstSubst_tm sigma_tm tau_tm theta_tm Eq_tm s0)
+        (compSubstSubst_tm (up_tm_tm sigma_tm) (up_tm_tm tau_tm)
+           (up_tm_tm theta_tm) (up_subst_subst_tm_tm _ _ _ Eq_tm) s1)
+  end.
 
-Lemma varL_tm   (sigmatm : ( fin ) -> tm ) : (funcomp) (subst_tm sigmatm) (var_tm ) = sigmatm .
-Proof. exact ((FunctionalExtensionality.functional_extensionality _ _ ) (fun x => eq_refl)). Qed.
+Lemma renRen_tm (xi_tm : nat -> nat) (zeta_tm : nat -> nat) (s : tm) :
+  ren_tm zeta_tm (ren_tm xi_tm s) = ren_tm (funcomp zeta_tm xi_tm) s.
+Proof.
+exact (compRenRen_tm xi_tm zeta_tm _ (fun n => eq_refl) s).
+Qed.
 
-Lemma varLRen_tm   (xitm : ( fin ) -> fin) : (funcomp) (ren_tm xitm) (var_tm ) = (funcomp) (var_tm ) xitm .
-Proof. exact ((FunctionalExtensionality.functional_extensionality _ _ ) (fun x => eq_refl)). Qed.
+Lemma renRen'_tm_pointwise (xi_tm : nat -> nat) (zeta_tm : nat -> nat) :
+  pointwise_relation _ eq (funcomp (ren_tm zeta_tm) (ren_tm xi_tm))
+    (ren_tm (funcomp zeta_tm xi_tm)).
+Proof.
+exact (fun s => compRenRen_tm xi_tm zeta_tm _ (fun n => eq_refl) s).
+Qed.
 
-Lemma compComp_tm    (sigmatm : ( fin ) -> tm ) (tautm : ( fin ) -> tm ) (s : tm ) : subst_tm tautm (subst_tm sigmatm s) = subst_tm ((funcomp) (subst_tm tautm) sigmatm) s .
-Proof. exact (compSubstSubst_tm sigmatm tautm (_) (fun n => eq_refl) s). Qed.
+Lemma renSubst_tm (xi_tm : nat -> nat) (tau_tm : nat -> tm) (s : tm) :
+  subst_tm tau_tm (ren_tm xi_tm s) = subst_tm (funcomp tau_tm xi_tm) s.
+Proof.
+exact (compRenSubst_tm xi_tm tau_tm _ (fun n => eq_refl) s).
+Qed.
 
-Lemma compComp'_tm    (sigmatm : ( fin ) -> tm ) (tautm : ( fin ) -> tm ) : (funcomp) (subst_tm tautm) (subst_tm sigmatm) = subst_tm ((funcomp) (subst_tm tautm) sigmatm) .
-Proof. exact ((FunctionalExtensionality.functional_extensionality _ _ ) (fun n => compComp_tm sigmatm tautm n)). Qed.
+Lemma renSubst_tm_pointwise (xi_tm : nat -> nat) (tau_tm : nat -> tm) :
+  pointwise_relation _ eq (funcomp (subst_tm tau_tm) (ren_tm xi_tm))
+    (subst_tm (funcomp tau_tm xi_tm)).
+Proof.
+exact (fun s => compRenSubst_tm xi_tm tau_tm _ (fun n => eq_refl) s).
+Qed.
 
-Lemma compRen_tm    (sigmatm : ( fin ) -> tm ) (zetatm : ( fin ) -> fin) (s : tm ) : ren_tm zetatm (subst_tm sigmatm s) = subst_tm ((funcomp) (ren_tm zetatm) sigmatm) s .
-Proof. exact (compSubstRen_tm sigmatm zetatm (_) (fun n => eq_refl) s). Qed.
+Lemma substRen_tm (sigma_tm : nat -> tm) (zeta_tm : nat -> nat) (s : tm) :
+  ren_tm zeta_tm (subst_tm sigma_tm s) =
+  subst_tm (funcomp (ren_tm zeta_tm) sigma_tm) s.
+Proof.
+exact (compSubstRen_tm sigma_tm zeta_tm _ (fun n => eq_refl) s).
+Qed.
 
-Lemma compRen'_tm    (sigmatm : ( fin ) -> tm ) (zetatm : ( fin ) -> fin) : (funcomp) (ren_tm zetatm) (subst_tm sigmatm) = subst_tm ((funcomp) (ren_tm zetatm) sigmatm) .
-Proof. exact ((FunctionalExtensionality.functional_extensionality _ _ ) (fun n => compRen_tm sigmatm zetatm n)). Qed.
+Lemma substRen_tm_pointwise (sigma_tm : nat -> tm) (zeta_tm : nat -> nat) :
+  pointwise_relation _ eq (funcomp (ren_tm zeta_tm) (subst_tm sigma_tm))
+    (subst_tm (funcomp (ren_tm zeta_tm) sigma_tm)).
+Proof.
+exact (fun s => compSubstRen_tm sigma_tm zeta_tm _ (fun n => eq_refl) s).
+Qed.
 
-Lemma renComp_tm    (xitm : ( fin ) -> fin) (tautm : ( fin ) -> tm ) (s : tm ) : subst_tm tautm (ren_tm xitm s) = subst_tm ((funcomp) tautm xitm) s .
-Proof. exact (compRenSubst_tm xitm tautm (_) (fun n => eq_refl) s). Qed.
+Lemma substSubst_tm (sigma_tm : nat -> tm) (tau_tm : nat -> tm) (s : tm) :
+  subst_tm tau_tm (subst_tm sigma_tm s) =
+  subst_tm (funcomp (subst_tm tau_tm) sigma_tm) s.
+Proof.
+exact (compSubstSubst_tm sigma_tm tau_tm _ (fun n => eq_refl) s).
+Qed.
 
-Lemma renComp'_tm    (xitm : ( fin ) -> fin) (tautm : ( fin ) -> tm ) : (funcomp) (subst_tm tautm) (ren_tm xitm) = subst_tm ((funcomp) tautm xitm) .
-Proof. exact ((FunctionalExtensionality.functional_extensionality _ _ ) (fun n => renComp_tm xitm tautm n)). Qed.
+Lemma substSubst_tm_pointwise (sigma_tm : nat -> tm) (tau_tm : nat -> tm) :
+  pointwise_relation _ eq (funcomp (subst_tm tau_tm) (subst_tm sigma_tm))
+    (subst_tm (funcomp (subst_tm tau_tm) sigma_tm)).
+Proof.
+exact (fun s => compSubstSubst_tm sigma_tm tau_tm _ (fun n => eq_refl) s).
+Qed.
 
-Lemma renRen_tm    (xitm : ( fin ) -> fin) (zetatm : ( fin ) -> fin) (s : tm ) : ren_tm zetatm (ren_tm xitm s) = ren_tm ((funcomp) zetatm xitm) s .
-Proof. exact (compRenRen_tm xitm zetatm (_) (fun n => eq_refl) s). Qed.
+Lemma rinstInst_up_tm_tm (xi : nat -> nat) (sigma : nat -> tm)
+  (Eq : forall x, funcomp (var_tm) xi x = sigma x) :
+  forall x, funcomp (var_tm) (upRen_tm_tm xi) x = up_tm_tm sigma x.
+Proof.
+exact (fun n =>
+       match n with
+       | S n' => ap (ren_tm shift) (Eq n')
+       | O => eq_refl
+       end).
+Qed.
 
-Lemma renRen'_tm    (xitm : ( fin ) -> fin) (zetatm : ( fin ) -> fin) : (funcomp) (ren_tm zetatm) (ren_tm xitm) = ren_tm ((funcomp) zetatm xitm) .
-Proof. exact ((FunctionalExtensionality.functional_extensionality _ _ ) (fun n => renRen_tm xitm zetatm n)). Qed.
+Fixpoint rinst_inst_tm (xi_tm : nat -> nat) (sigma_tm : nat -> tm)
+(Eq_tm : forall x, funcomp (var_tm) xi_tm x = sigma_tm x) (s : tm) {struct s}
+   : ren_tm xi_tm s = subst_tm sigma_tm s :=
+  match s with
+  | var_tm s0 => Eq_tm s0
+  | Univ s0 => congr_Univ (eq_refl s0)
+  | Lam s0 s1 =>
+      congr_Lam (rinst_inst_tm xi_tm sigma_tm Eq_tm s0)
+        (rinst_inst_tm (upRen_tm_tm xi_tm) (up_tm_tm sigma_tm)
+           (rinstInst_up_tm_tm _ _ Eq_tm) s1)
+  | App s0 s1 s2 s3 =>
+      congr_App (rinst_inst_tm xi_tm sigma_tm Eq_tm s0)
+        (rinst_inst_tm (upRen_tm_tm xi_tm) (up_tm_tm sigma_tm)
+           (rinstInst_up_tm_tm _ _ Eq_tm) s1)
+        (rinst_inst_tm xi_tm sigma_tm Eq_tm s2)
+        (rinst_inst_tm xi_tm sigma_tm Eq_tm s3)
+  | Pi s0 s1 =>
+      congr_Pi (rinst_inst_tm xi_tm sigma_tm Eq_tm s0)
+        (rinst_inst_tm (upRen_tm_tm xi_tm) (up_tm_tm sigma_tm)
+           (rinstInst_up_tm_tm _ _ Eq_tm) s1)
+  end.
 
-End tm.
+Lemma rinstInst'_tm (xi_tm : nat -> nat) (s : tm) :
+  ren_tm xi_tm s = subst_tm (funcomp (var_tm) xi_tm) s.
+Proof.
+exact (rinst_inst_tm xi_tm _ (fun n => eq_refl) s).
+Qed.
 
+Lemma rinstInst'_tm_pointwise (xi_tm : nat -> nat) :
+  pointwise_relation _ eq (ren_tm xi_tm) (subst_tm (funcomp (var_tm) xi_tm)).
+Proof.
+exact (fun s => rinst_inst_tm xi_tm _ (fun n => eq_refl) s).
+Qed.
 
+Lemma instId'_tm (s : tm) : subst_tm (var_tm) s = s.
+Proof.
+exact (idSubst_tm (var_tm) (fun n => eq_refl) s).
+Qed.
 
+Lemma instId'_tm_pointwise : pointwise_relation _ eq (subst_tm (var_tm)) id.
+Proof.
+exact (fun s => idSubst_tm (var_tm) (fun n => eq_refl) s).
+Qed.
 
+Lemma rinstId'_tm (s : tm) : ren_tm id s = s.
+Proof.
+exact (eq_ind_r (fun t => t = s) (instId'_tm s) (rinstInst'_tm id s)).
+Qed.
 
+Lemma rinstId'_tm_pointwise : pointwise_relation _ eq (@ren_tm id) id.
+Proof.
+exact (fun s => eq_ind_r (fun t => t = s) (instId'_tm s) (rinstInst'_tm id s)).
+Qed.
 
+Lemma varL'_tm (sigma_tm : nat -> tm) (x : nat) :
+  subst_tm sigma_tm (var_tm x) = sigma_tm x.
+Proof.
+exact (eq_refl).
+Qed.
 
+Lemma varL'_tm_pointwise (sigma_tm : nat -> tm) :
+  pointwise_relation _ eq (funcomp (subst_tm sigma_tm) (var_tm)) sigma_tm.
+Proof.
+exact (fun x => eq_refl).
+Qed.
 
+Lemma varLRen'_tm (xi_tm : nat -> nat) (x : nat) :
+  ren_tm xi_tm (var_tm x) = var_tm (xi_tm x).
+Proof.
+exact (eq_refl).
+Qed.
 
+Lemma varLRen'_tm_pointwise (xi_tm : nat -> nat) :
+  pointwise_relation _ eq (funcomp (ren_tm xi_tm) (var_tm))
+    (funcomp (var_tm) xi_tm).
+Proof.
+exact (fun x => eq_refl).
+Qed.
 
+Class Up_tm X Y :=
+    up_tm : X -> Y.
 
-Global Instance Subst_tm   : Subst1 (( fin ) -> tm ) (tm ) (tm ) := @subst_tm   .
+#[global] Instance Subst_tm : (Subst1 _ _ _) := @subst_tm.
 
-Global Instance Ren_tm   : Ren1 (( fin ) -> fin) (tm ) (tm ) := @ren_tm   .
+#[global] Instance Up_tm_tm : (Up_tm _ _) := @up_tm_tm.
 
-Global Instance VarInstance_tm  : Var (fin) (tm ) := @var_tm  .
+#[global] Instance Ren_tm : (Ren1 _ _ _) := @ren_tm.
 
-Notation "x '__tm'" := (var_tm x) (at level 5, format "x __tm") : subst_scope.
+#[global]
+Instance VarInstance_tm : (Var _ _) := @var_tm.
 
-Notation "x '__tm'" := (@ids (_) (_) VarInstance_tm x) (at level 5, only printing, format "x __tm") : subst_scope.
+Notation "[ sigma_tm ]" := (subst_tm sigma_tm)
+( at level 1, left associativity, only printing)  : fscope.
 
-Notation "'var'" := (var_tm) (only printing, at level 1) : subst_scope.
+Notation "s [ sigma_tm ]" := (subst_tm sigma_tm s)
+( at level 7, left associativity, only printing)  : subst_scope.
 
-Class Up_tm X Y := up_tm : ( X ) -> Y.
+Notation "↑__tm" := up_tm (only printing)  : subst_scope.
 
-Notation "↑__tm" := (up_tm) (only printing) : subst_scope.
+Notation "↑__tm" := up_tm_tm (only printing)  : subst_scope.
 
-Notation "↑__tm" := (up_tm_tm) (only printing) : subst_scope.
+Notation "⟨ xi_tm ⟩" := (ren_tm xi_tm)
+( at level 1, left associativity, only printing)  : fscope.
 
-Global Instance Up_tm_tm   : Up_tm (_) (_) := @up_tm_tm   .
+Notation "s ⟨ xi_tm ⟩" := (ren_tm xi_tm s)
+( at level 7, left associativity, only printing)  : subst_scope.
 
-Notation "s [ sigmatm ]" := (subst_tm sigmatm s) (at level 7, left associativity, only printing) : subst_scope.
+Notation "'var'" := var_tm ( at level 1, only printing)  : subst_scope.
 
-Notation "[ sigmatm ]" := (subst_tm sigmatm) (at level 1, left associativity, only printing) : fscope.
+Notation "x '__tm'" := (@ids _ _ VarInstance_tm x)
+( at level 5, format "x __tm", only printing)  : subst_scope.
 
-Notation "s ⟨ xitm ⟩" := (ren_tm xitm s) (at level 7, left associativity, only printing) : subst_scope.
+Notation "x '__tm'" := (var_tm x) ( at level 5, format "x __tm")  :
+subst_scope.
 
-Notation "⟨ xitm ⟩" := (ren_tm xitm) (at level 1, left associativity, only printing) : fscope.
+#[global]
+Instance subst_tm_morphism :
+ (Proper (respectful (pointwise_relation _ eq) (respectful eq eq))
+    (@subst_tm)).
+Proof.
+exact (fun f_tm g_tm Eq_tm s t Eq_st =>
+       eq_ind s (fun t' => subst_tm f_tm s = subst_tm g_tm t')
+         (ext_tm f_tm g_tm Eq_tm s) t Eq_st).
+Qed.
 
-Ltac auto_unfold := repeat unfold subst1,  subst2,  Subst1,  Subst2,  ids,  ren1,  ren2,  Ren1,  Ren2,  Subst_tm,  Ren_tm,  VarInstance_tm.
+#[global]
+Instance subst_tm_morphism2 :
+ (Proper (respectful (pointwise_relation _ eq) (pointwise_relation _ eq))
+    (@subst_tm)).
+Proof.
+exact (fun f_tm g_tm Eq_tm s => ext_tm f_tm g_tm Eq_tm s).
+Qed.
 
-Tactic Notation "auto_unfold" "in" "*" := repeat unfold subst1,  subst2,  Subst1,  Subst2,  ids,  ren1,  ren2,  Ren1,  Ren2,  Subst_tm,  Ren_tm,  VarInstance_tm in *.
+#[global]
+Instance ren_tm_morphism :
+ (Proper (respectful (pointwise_relation _ eq) (respectful eq eq)) (@ren_tm)).
+Proof.
+exact (fun f_tm g_tm Eq_tm s t Eq_st =>
+       eq_ind s (fun t' => ren_tm f_tm s = ren_tm g_tm t')
+         (extRen_tm f_tm g_tm Eq_tm s) t Eq_st).
+Qed.
 
-Ltac asimpl' := repeat first [progress rewrite ?instId_tm| progress rewrite ?compComp_tm| progress rewrite ?compComp'_tm| progress rewrite ?rinstId_tm| progress rewrite ?compRen_tm| progress rewrite ?compRen'_tm| progress rewrite ?renComp_tm| progress rewrite ?renComp'_tm| progress rewrite ?renRen_tm| progress rewrite ?renRen'_tm| progress rewrite ?varL_tm| progress rewrite ?varLRen_tm| progress (unfold up_ren, upRen_tm_tm, up_tm_tm)| progress (cbn [subst_tm ren_tm])| fsimpl].
+#[global]
+Instance ren_tm_morphism2 :
+ (Proper (respectful (pointwise_relation _ eq) (pointwise_relation _ eq))
+    (@ren_tm)).
+Proof.
+exact (fun f_tm g_tm Eq_tm s => extRen_tm f_tm g_tm Eq_tm s).
+Qed.
 
-Ltac asimpl := repeat try unfold_funcomp; auto_unfold in *; asimpl'; repeat try unfold_funcomp.
+Ltac auto_unfold := repeat
+                     unfold VarInstance_tm, Var, ids, Ren_tm, Ren1, ren1,
+                      Up_tm_tm, Up_tm, up_tm, Subst_tm, Subst1, subst1.
+
+Tactic Notation "auto_unfold" "in" "*" := repeat
+                                           unfold VarInstance_tm, Var, ids,
+                                            Ren_tm, Ren1, ren1, Up_tm_tm,
+                                            Up_tm, up_tm, Subst_tm, Subst1,
+                                            subst1 in *.
+
+Ltac asimpl' := repeat (first
+                 [ progress setoid_rewrite substSubst_tm_pointwise
+                 | progress setoid_rewrite substSubst_tm
+                 | progress setoid_rewrite substRen_tm_pointwise
+                 | progress setoid_rewrite substRen_tm
+                 | progress setoid_rewrite renSubst_tm_pointwise
+                 | progress setoid_rewrite renSubst_tm
+                 | progress setoid_rewrite renRen'_tm_pointwise
+                 | progress setoid_rewrite renRen_tm
+                 | progress setoid_rewrite varLRen'_tm_pointwise
+                 | progress setoid_rewrite varLRen'_tm
+                 | progress setoid_rewrite varL'_tm_pointwise
+                 | progress setoid_rewrite varL'_tm
+                 | progress setoid_rewrite rinstId'_tm_pointwise
+                 | progress setoid_rewrite rinstId'_tm
+                 | progress setoid_rewrite instId'_tm_pointwise
+                 | progress setoid_rewrite instId'_tm
+                 | progress unfold up_tm_tm, upRen_tm_tm, up_ren
+                 | progress cbn[subst_tm ren_tm]
+                 | progress fsimpl ]).
+
+Ltac asimpl := check_no_evars;
+                repeat
+                 unfold VarInstance_tm, Var, ids, Ren_tm, Ren1, ren1,
+                  Up_tm_tm, Up_tm, up_tm, Subst_tm, Subst1, subst1 in *;
+                asimpl'; minimize.
 
 Tactic Notation "asimpl" "in" hyp(J) := revert J; asimpl; intros J.
 
-Tactic Notation "auto_case" := auto_case (asimpl; cbn; eauto).
+Tactic Notation "auto_case" := auto_case ltac:(asimpl; cbn; eauto).
 
-Tactic Notation "asimpl" "in" "*" := auto_unfold in *; repeat first [progress rewrite ?instId_tm in *| progress rewrite ?compComp_tm in *| progress rewrite ?compComp'_tm in *| progress rewrite ?rinstId_tm in *| progress rewrite ?compRen_tm in *| progress rewrite ?compRen'_tm in *| progress rewrite ?renComp_tm in *| progress rewrite ?renComp'_tm in *| progress rewrite ?renRen_tm in *| progress rewrite ?renRen'_tm in *| progress rewrite ?varL_tm in *| progress rewrite ?varLRen_tm in *| progress (unfold up_ren, upRen_tm_tm, up_tm_tm in *)| progress (cbn [subst_tm ren_tm] in *)| fsimpl in *].
+Ltac substify := auto_unfold; try setoid_rewrite rinstInst'_tm_pointwise;
+                  try setoid_rewrite rinstInst'_tm.
 
-Ltac substify := auto_unfold; try repeat (erewrite rinstInst_tm).
+Ltac renamify := auto_unfold; try setoid_rewrite_left rinstInst'_tm_pointwise;
+                  try setoid_rewrite_left rinstInst'_tm.
 
-Ltac renamify := auto_unfold; try repeat (erewrite <- rinstInst_tm).
+End Core.
+
+Module Extra.
+
+Import Core.
+
+#[global] Hint Opaque subst_tm: rewrite.
+
+#[global] Hint Opaque ren_tm: rewrite.
+
+End Extra.
+
+Module interface.
+
+Export Core.
+
+Export Extra.
+
+End interface.
+
+Export interface.
 
