theories/imports.v
@@ -6,9 +6,12 @@ From Hammer Require Export Tactics.
 Require Export Psatz.
 
 Global Set Warnings "-notation-overridden".
-Require Export Autosubst2.syntax.
+Require Export Autosubst2.syntax Autosubst2.unscoped Autosubst2.core.
 
 Notation "s [ sigmatm ]" := (subst_tm sigmatm s) (at level 7, left associativity) : subst_scope.
 Notation "s ⟨ xitm ⟩" := (ren_tm xitm s) (at level 7, left associativity) : subst_scope.
+Notation "s '..'" := (scons s ids) (at level 1, format "s ..") : subst_scope.
+Import List.ListNotations.
 
-Global Open Scope subst_scope. 
+Global Open Scope list_scope.
+Global Open Scope subst_scope.
